examples/graph/theories/HeapEquiv.v
@@ -1,0 +1,25 @@
+(*Contains only the rewriting Lemma for [toList] of Heap because it takes forever to compile*)
+Require Import Data.Graph.Inductive.Internal.Heap.
+Require Import Coq.Program.Wf.
+
+
+Section Heap.
+
+Context {A B : Type} `{Hord: Base.Ord A} {Hdefault : Err.Default A} {Hdefault' : Err.Default B}.
+
+Definition expand_toList := 
+  fun {a} {b} `{GHC.Base.Ord a} `{Err.Default (a * b)} (arg_0__ : Heap a b) =>
+    match arg_0__ with
+    | Heap.Empty => nil
+    | h => let 'pair x r := pair (findMin h) (deleteMin h) in cons x (toList r)
+    end.
+
+Lemma unfold_toList : forall h, expand_toList h = toList h.
+Proof.
+  intros. destruct h; simpl. reflexivity. simpl.  f_equal. unfold toList at 2. unfold toList_func.
+  rewrite fix_sub_eq; simpl.  reflexivity. intros. destruct x; simpl. destruct s; simpl. destruct s; simpl. destruct s; simpl.
+  destruct s eqn : ?; simpl. destruct h eqn : ?. reflexivity. f_equal. rewrite H0. reflexivity.
+Qed.
+
+End Heap.
+
