examples/graph/theories/HeapProofs.v
@@ -1,0 +1,128 @@
+Require Import Data.Graph.Inductive.Internal.Heap.
+Require Import Coq.Lists.List.
+Require Import Coq.Wellfounded.Inverse_Image.
+Require Import Omega.
+Require Import HeapEquiv.
+
+Require Import Equations.Equations.
+
+Section Heap.
+
+Context {A B : Type} `{Hord: Base.Ord A} {Hdefault : Err.Default A} {Hdefault' : Err.Default B}.
+
+
+(*An equivalent version that uses Equations*)
+
+Equations toList' {a} {b} `{GHC.Base.Ord a} `{Err.Default (a * b)} (h: Heap a b) : list (a * b) by wf (size h) lt :=
+toList' h => match h with 
+              | Heap.Empty => nil 
+              | h' => let 'pair x r := pair (findMin h') (deleteMin h') in cons x (toList r)
+              end. 
+
+(*Better induction for heaps (from CPDT)*)
+
+Section All.
+  Variable T : Type.
+  Variable P : T -> Prop.
+
+  Fixpoint All (ls : list T) : Prop :=
+    match ls with
+      | nil => True
+      | cons h t => P h /\ All t
+    end.
+End All.
+
+Section Heap_ind'.
+  Variable P : (Heap A B) -> Prop.
+
+  Hypothesis Node_case : forall a b (ls : list (Heap A B)),
+    All (Heap A B) P ls -> P (Node a b ls).
+
+  Hypothesis Empty_case :  P Heap.Empty.
+
+  Fixpoint Heap_ind' (tr : (Heap A B)) : P tr :=
+    match tr with
+      | Node a b ls => Node_case a b ls
+        ((fix list_nat_tree_ind (ls : list (Heap A B)) : All (Heap A B) P ls :=
+          match ls  with
+            | nil => I
+            | cons tr' rest => conj (Heap_ind' tr') (list_nat_tree_ind rest)
+          end) ls)
+      | Empty => Empty_case
+    end.
+
+End Heap_ind'.
+
+(*Now we can work with Equations version instead, which might be easier*)
+Lemma toList_equiv: forall h,
+  toList h = toList' h.
+Proof.
+  intros. rewrite <- unfold_toList. eapply toList'_elim. intros. destruct h0. simpl.
+  reflexivity. simpl. reflexivity.
+Qed.
+
+(*In the heap*)
+Fixpoint In_Heap  (p : A * B) (h: Heap A B) :=
+  match h with
+  | Heap.Empty => False
+  | Node x y l => (x,y) = p \/ List.fold_right (fun y acc => y \/ acc) False (List.map (fun y => In_Heap p y) l)
+  end.
+
+(*Specifications for different functions*)
+Lemma in_heap_merge: forall p h1 h2,
+  In_Heap p (merge h1 h2) <-> In_Heap p h1 \/ In_Heap p h2.
+Proof.
+  intros. unfold merge. generalize dependent h2. 
+  induction h1 using Heap_ind'.
+  - intros. destruct h2. simpl. split; intros. left. assumption. destruct H1; try assumption. destruct H1.
+    destruct (Base.op_zl__ a a0) eqn : ?.
+    + simpl. split; intros. destruct H1. left. left. assumption. destruct H1. destruct H1.
+      right. left. assumption. right. right. assumption. left. right. assumption.
+      destruct H1. destruct H1. left. assumption. right. right. assumption.
+      destruct H1. right. left. left. assumption. right. left. right. assumption.
+    + simpl. split; intros. destruct H1. right. left. assumption. destruct H1. destruct H1.
+      left. left. assumption. left. right. assumption. right. right. assumption.
+      destruct H1. destruct H1. right. left. left. assumption. right. left. right. assumption.
+      destruct H1. left. assumption. right. right. assumption.
+  - intros. simpl. destruct h2. split; intros; simpl in *. auto. destruct H0; auto. split; intros.
+    right. assumption. destruct H0. destruct H0. assumption.
+Qed.
+
+Lemma in_heap_mergeAll: forall p hs,
+  In_Heap p (mergeAll hs) <-> fold_right (fun x acc => In_Heap p x \/ acc) False hs.
+Proof.
+  intros. induction hs using (well_founded_induction
+                     (wf_inverse_image _ nat _ (@length _)
+                        PeanoNat.Nat.lt_wf_0)).
+  destruct hs. simpl. reflexivity. simpl. destruct hs.
+  simpl. split; intros. left. assumption. destruct H1. assumption. destruct H1.
+  split; intros. apply in_heap_merge in H1. destruct H1. apply in_heap_merge in H1.
+  destruct H1. left. assumption. simpl. right. left. assumption. 
+  right. apply H0 in H1. simpl. right. apply H1. simpl. omega.
+  rewrite in_heap_merge. rewrite in_heap_merge. simpl in H1. destruct H1.
+  left. left. assumption. destruct H1. left. right. assumption. 
+  right. apply H0. simpl. omega. assumption.
+Qed.
+
+Program Instance triple : Err.Default (A * B * Heap A B).
+Next Obligation.
+inversion Hdefault. inversion Hdefault'. apply (default, default0, Heap.Empty).
+Defined.
+
+Lemma in_heap_splitMin: forall (p: A * B) (h h': Heap A B) k v,
+  h <> Heap.Empty ->
+  splitMin h = (k, v, h') ->
+  In_Heap p h <-> p = (k,v) \/ In_Heap p h'.
+Proof.
+  intros. unfold splitMin in H1. destruct h. contradiction. inversion H1; subst.
+  rewrite in_heap_mergeAll. simpl.
+  assert (forall l' p,
+  fold_right (fun y acc : Prop => y \/ acc) False (map (fun y : Heap A B => In_Heap p y) l') <->
+  fold_right (fun (x : Heap A B) (acc : Prop) => In_Heap p x \/ acc) False l'). { intros; induction l'.
+  simpl. reflexivity. simpl. split; intros. destruct H2. left. assumption. right. apply IHl'. apply H2.
+  destruct H2. left. assumption. right. apply IHl'. apply H2. } rewrite H2. split; intros.
+  destruct H3. left. subst. reflexivity. right. assumption. destruct H3. left. subst. reflexivity. right.
+  assumption.
+Qed.
+
+End Heap.
