examples/graph/theories/Lex.v
@@ -1,0 +1,68 @@
+Require Import Coq.Relations.Relation_Operators.
+Require Import Relation_Operators.
+Require Import Coq.Relations.Relation_Definitions.
+Require Import Coq.Wellfounded.Lexicographic_Product.
+Require Import Coq.Classes.RelationClasses.
+Require Import Omega.
+
+
+Definition compose A (R S : relation A) : relation A :=
+  fun x y => exists z, R x z /\ S z y.
+(*Heavily based on the Lex proofs from the CoLoR library. The main difference is that I need the 
+  first relation to be on the second type in the tuple because of the order of the arguments in the
+  Haskell functions*)
+Section Lex.
+  Variables (A B : Type) (ltA eqA : relation A) (ltB : relation B).
+  Inductive lex : relation (B * A) :=
+  | lex1 a a' b b' : ltA a a' -> lex (b,a) (b',a')
+  | lex2 a a' b b' : eqA a a' -> ltB b b' -> lex (b,a) (b',a').
+  Variables (WF_gtA : well_founded ltA) (WF_gtB : well_founded ltB)
+    (eqA_trans : Transitive eqA) (Hcomp : forall x y : A, (exists z : A, eqA y z /\ ltA x z) -> ltA x y)
+    (eqA_sym: Symmetric eqA).
+  
+   Lemma lex_Acc_eq : forall a b,
+    Acc lex (b,a) -> forall a', eqA a a' -> Acc lex (b,a').
+
+  Proof.
+    intros a b SN_ab a' eqaa'. inversion SN_ab. apply Acc_intro.
+    destruct y as (a'',b'). intro H'.
+    inversion H'; subst a'0 b'0 a0 b0; apply H.
+    apply lex1. apply Hcomp. exists a'. auto. 
+    apply lex2. assert (eqA a' b'). eapply eqA_sym. assumption. 
+    pose proof (eqA_trans _ _ _ eqaa' H0). apply eqA_sym. assumption. assumption.
+  Qed.
+
+  Lemma lex_Acc :
+    forall a, Acc ltA a -> forall b, Acc ltB b -> Acc lex (b, a).
+
+  Proof.
+    induction 1 as [a Ha1 Ha2]. induction 1 as [b Hb1 Hb2]. apply Acc_intro.
+    destruct y as (a'',b'). intro H. inversion H. subst a'' b'0. subst a0. subst a'. (* subst a'' b'0 a0 b0.*)
+    (* gtA a a' *)
+    apply Ha2. exact H1. apply WF_gtB. 
+    (* eqA a a' /\ gtB b b' *)
+    apply (@lex_Acc_eq a).
+    apply Hb2. assumption. apply eqA_sym. assumption.
+  Qed.
+
+  Lemma WF_lex : well_founded lex.
+
+  Proof.
+    unfold well_founded. destruct a as (a,b). apply lex_Acc. apply WF_gtA. apply WF_gtB.
+  Qed.
+
+End Lex.
+
+Definition f_nat_lt {a} (f: a -> nat) x y := f x < f y.
+
+Lemma f_nat_lt_acc: forall {a} (f: a -> nat) x n, f x <= n -> Acc (f_nat_lt f) x.
+Proof.
+  intros. generalize dependent x. induction n; auto.
+  - intros. apply Acc_intro. intros. unfold f_nat_lt in *. omega.
+  - unfold f_nat_lt in *. intros. apply Acc_intro. intros. apply IHn. omega.
+Qed.
+
+Lemma f_nat_lt_wf: forall {a} (f: a -> nat), well_founded (f_nat_lt f).
+Proof.
+  red. intro. intro. intro. eapply f_nat_lt_acc. eauto.
+Qed.
